\documentclass{beamer}

\input{prelim}

%\AtBeginSection[]
%{
%  \begin{frame}
%    \frametitle{Table of Contents}
%    \tableofcontents[currentsection]
%  \end{frame}
%}

\title{\K Summarizer: Foundations}
\author{Runtime Verification, Inc.}

\begin{document}

\frame{\titlepage}

\begin{frame}
\frametitle{Purpose}
Formalize the key concepts of the \K summarizer in matching logic.
\begin{itemize}
\item \K control-flow graphs
\item Basic blocks
\item Soundness and completeness
\end{itemize}
We work under the following assumptions:
\begin{itemize}
\item Formal semantics are deterministic
  (i.e., $\vdash \onext \varphi \imp \anext \varphi$)
\item All patterns are constrained terms: $t \land p$
\end{itemize}
\end{frame}

\begin{frame}
\frametitle{\K Control-Flow Graphs}
\begin{definition}
A \K control-flow graph (abbreviated KCFG) $G = (V, \Er, \Ea, \Es)$ is a finite directed graph
with three types of edges where
\begin{itemize}
\item the vertex set $V$ is a set of constrained terms;
\item $\Er \subseteq V \times V$ is called the \emph{rewriting relation};
\item $\Ea \subseteq V \times V$ is called the \emph{abstracting relation};
\item $\Es \subseteq V \times V$ is called the \emph{splitting relation}. 
\end{itemize}
We write $\varphi \tor \psi$ 
($\varphi \toa \psi$ and $\varphi \tos \psi$, resp.)
for the three types of edges.
\end{definition}
\end{frame}

\begin{frame}
\frametitle{Rewriting Edges}
$t_1 \land p_1 \tor t_2 \land p_2$ means
\begin{itemize}
\item finite- and at-least-one-step rewriting 
      \begin{equation}\label{eq:tor}
      \vdash t_1 \land p_1 \imp \onext \eventually (t_2 \land p_2)
      \end{equation}
\item $\eventually \varphi \equiv \mu X \ld \varphi \lor \onext X$
\item The next symbol $\onext$ enforces ``at-least-one-step''
\item Thanks to determinism, we can just use the ``one-path'' operators
      $\onext$ and $\eventually$.
\item \Cref{eq:tor} specifies a basic block.
\begin{itemize}
\item All the concrete instances of $t_1 \land p_1$ are covered:
\[\vdash \forall \bar{x}
   \ld \left( t_1 \land p_1 \imp \onext \eventually (t_2 \land p_2) \right)\]
\item Not getting stuck somewhere in the middle.
\item Determinism (by assumption)
\end{itemize}
\end{itemize}
\end{frame}

\begin{frame}
\frametitle{Abstracting Edges}
$t_1 \land p_1 \toa t_2 \land p_2$ means
\begin{itemize}
\item implication
      \begin{equation}\label{eq:toa}
      \vdash t_1 \land p_1 \imp \exists \bar{y} \ld t_2 \land p_2
      \end{equation}
      where $\bar{y} = \FV{rhs} \setminus \FV{lhs}$
\item The most common case is when
      $t_1 \equiv t_2[\bar{y}]_{\bar{p}}$ where $\bar{p}$ are the positions of $\bar{y}$ in $t_2$
\item It means that \Cref{eq:toa} has a witness substitution
      \[\pi = [t_{11} / y_1 \dots t_{1n} / y_n]\]
\item $t_1 \land p_1 \toa^\pi t_2 \land p_2$
\end{itemize}
\end{frame}

\begin{frame}
\frametitle{Splitting Edges}
$t \land p \tos t \land (p \land q_i)$ for $i = 1, 2, \dots, n$
\begin{itemize}
\item Complete Cases: $\vdash q_1 \lor \dots \lor q_n$
\item $t \land p \tos^{q_i} t \land (p \land q_i)$
\end{itemize}
\end{frame}

\begin{frame}
\frametitle{Review}
A KCFG $G = (V, \Er, \Ea, \Es)$ has
\begin{itemize}
\item V: a set of constrained terms (nodes)
\item $t_1 \land p_1 \tor t_2 \land p_2$: 
      basic block ($\ge 1$ steps)
\item $t \land p \tor^\pi t_2 \land p$ with a witness substitution $\pi$
\item $t \land p \tor^{q_i} t \land (p \land q_i)$ with a condition $q_i$
\begin{itemize}
\item $\vdash q_1 \lor \dots \lor q_n$
\end{itemize}
\end{itemize}
Termination Condition
\begin{itemize}
\item $\Phi_T$: a (user-provided) termination pattern\\
if not provided, $\Phi_T$ is $\anext \bot$ (e.g., when \code{<k>\,.\,</k>})
\item $t \land p$ has no successors iff $\vdash t \land p \imp \Phi_T$
\end{itemize}
\end{frame}

\begin{frame}
\frametitle{Semantics Derived from a KCFG}
Given a KCFG $G = (V, \Er, \Ea, \Es)$, we derive a new semantics
\begin{itemize}
\item for every $\varphi_1 \tos^{q} \varphi_2 \tor \varphi_3$, add
      \[ \text{rule} \quad \varphi_1 \To \varphi_3 \quad \text{requires} \  q\]
\item Let $\Gamma^G$ be the set of derived semantic rules.
\end{itemize}
\begin{theorem}
For any $t$ and its KCFG $G^t$, 
\[\Gamma^L \vdash t \To t' \quad\text{iff}\quad
  \Gamma^{G^t} \vdash t \To t'\]
\end{theorem}
\end{frame}

\end{document}